\documentclass[plain]{pset}
\usepackage{dylanhu}

\title{Homework 2}
\author{Dylan Hu}
\prof{Professor Zhuolun Yang}
\course{APMA 0360 --- Partial Differential Equations}
\date{February 18, 2024}

\begin{document}

\maketitle

\pagebreak

\begin{problem}
Let \(a\) and \(c\) be real numbers.
\begin{enumerate}[label = (\alph*)]
    \item Show that if \(g(x) = f(x - a)\), then \(\hat{g}(k) = e^{ika}\hat{f}(k)\).
    \item Use the Fourier transform and part (a) to solve the transport PDE
          \[
              \begin{cases}
                  u_t + cu_x = 0 \\
                  u(x, 0) = f(x)
              \end{cases}
          \]
\end{enumerate}
\end{problem}
\begin{solution}
    \[\]
    \vspace*{-4em}
    \begin{enumerate}[label = (\alph*)]
        \item
              \begin{align*}
                  \hat{g}(k) & = \int_{-\infty}^{\infty} g(x)e^{-ikx}dx                                        \\
                             & = \int_{-\infty}^{\infty} f(x - a)e^{-ikx}dx                                    \\
                             & = \int_{-\infty}^{\infty} f(y)e^{-ik(y + a)}dy \quad \text{(let \(y = x - a\))} \\
                             & = e^{ika}\int_{-\infty}^{\infty} f(y)e^{-iky}dy                                 \\
                             & = e^{ika}\hat{f}(k).
              \end{align*}
        \item \begin{align*}
                  u_t(x, t)       & = -cu_x(x, t)                                                                                           \\
                  \hat{u}_t(k, t) & = \int_{-\infty}^{\infty} -cu_x(x, t)e^{-ikx}dx                                                         \\
                                  & = -c\int_{-\infty}^{\infty} u_x(x, t)e^{-ikx}dx                                                         \\
                                  & = -c{\left[ u(x, t)e^{-ikx} \right]}_{-\infty}^{\infty} + c\int_{-\infty}^{\infty} u(x, t)ik e^{-ikx}dx \\
                                  & = cik\hat{u}(k, t).
              \end{align*}
              We have the ODE \(\hat{u}_t(k, t) = cik\hat{u}(k, t)\), which has the solution \(\hat{u}(k, t) = \hat{u}(k, 0)e^{cikt} = \hat{f}(k)e^{cikt}\).

              Using part (a), we have
              \[u(x, t) = f(x - ct)\]
              which is the solution to the transport PDE\@.
    \end{enumerate}
\end{solution}

\pagebreak

\begin{problem}
Consider the heat equation \(u_t = Du_{xx}\) with \(x \in \mathbb{R}\) and \(D > 0\).
\begin{enumerate}[label = (\alph*)]
    \item For each \(k \in \mathbb{R}\), find \(\lambda = \lambda(k) \in \mathbb{R}\) so that \(u(x, t) = e^{\lambda t}e^{ikx}\) satisfies the heat equation. Here \(i\) = \(\sqrt{-1}\).
    \item Assume that \(a(k)\) is Schwartz class in \(k\). Show that \(u(x, t) = \int_{-\infty}^{\infty} a(k)e^{\lambda(k)t}e^{ikx}dk\) satisfies the heat equation for \(t \geq 0\).
\end{enumerate}
\end{problem}
\begin{solution}
    \[\]
    \vspace*{-4em}
    \begin{enumerate}[label = (\alph*)]
        \item \begin{align*}
                  u_t(x, t)    & = \frac{\partial}{\partial t}e^{\lambda t}e^{ikx}     \\
                               & = \lambda e^{\lambda t}e^{ikx}                        \\
                  u_{xx}(x, t) & = \frac{\partial^2}{\partial x^2}e^{\lambda t}e^{ikx} \\
                               & = -k^2e^{\lambda t}e^{ikx}.
              \end{align*}
              \[u_t(x, t) = Du_{xx}(x, t) \implies \lambda e^{\lambda t}e^{ikx} = -Dk^2e^{\lambda t}e^{ikx}.\]
              \[\lambda(k) = -Dk^2.\]
        \item \[u_t(x, t) = \int_{-\infty}^{\infty} a(k)\lambda(k)e^{\lambda(k)t}e^{ikx}dk = \int_{-\infty}^{\infty} a(k)(-Dk^2)e^{-Dk^2t}e^{ikx}dk.\]
              \[u_{xx}(x, t) = \int_{-\infty}^{\infty} a(k)(-k^2)e^{-Dk^2t}e^{ikx}dk.\]
              \[u_t(x, t) = Du_{xx}(x, t).\]
              Note that \(t \geq 0\) so that \(e^{-Dk^2t}\) is either 1 or Schwartz class.

              Thus, \(u(x, t) = \int_{-\infty}^{\infty} a(k)e^{\lambda(k)t}e^{ikx}dk\) satisfies the heat equation for \(t \geq 0\).
    \end{enumerate}
\end{solution}

\pagebreak

\begin{problem}
Consider the equation \(u_t = u_{xxxx}\) for \(x \in \mathbb{R}\) with \(u(x,0) = f(x)\) where \(f(x)\) is Schwartz class. Derive an expression for the Fourier transform \(\hat{u}(k, t)\) of the solution \(u(x, t)\) in terms of \(k\), \(t\), and \(\hat{f}(k)\). (You do not need to find \(u(x, t)\) from \(\hat{u}(k, t)\)).
\end{problem}
\begin{solution}
    \begin{align*}
        u_t(x, t)       & = u_{xxxx}(x, t)                                     \\
        \hat{u}_t(k, t) & = \int_{-\infty}^{\infty} u_{xxxx}(x, t)e^{-ikx}dx   \\
                        & = \int_{-\infty}^{\infty} u(x, t){(-ik)}^4e^{-ikx}dx \\
                        & = {(-ik)}^4\hat{u}(k, t)                             \\
                        & = k^4\hat{u}(k, t).
    \end{align*}
    We have the ODE \(\hat{u}_t(k, t) = k^4\hat{u}(k, t)\), which has the solution \(\hat{u}(k, t) = \hat{u}(k, 0)e^{k^4t} = \hat{f}(k)e^{k^4t}\).

\end{solution}

\pagebreak

\begin{problem}
\[\]
\vspace*{-4em}
\begin{enumerate}[label = (\alph*)]
    \item For given \(D > 0\) and \(a, c \in \mathbb{R}\), consider the equation \(u_t = Du_{xx} + cu_x - au\) for \(x \in \mathbb{R}\) and \(t > 0\). Assume that \(u(x, t)\) is a solution of this equation. Verify that \(v(x, t) \coloneqq u(y - ct, t)e^{at}\) is a solution of \(v_t = Dv_{yy}\) for \(y \in \mathbb{R}\) and \(t > 0\).
    \item Recall that (from HW1)
          \[v(y, t) = \frac{1}{\sqrt{4\pi t}}e^{-\frac{y^2}{4t}}\]
          satisfies \(v_t = v_{yy}\) for \(y \in \mathbb{R}\) and \(t > 0\). Use the preceding part to find the solution \(u(x, t)\) to \(u_t = u_{xx} + 2u_x - 0.5u\).
\end{enumerate}
\end{problem}
\begin{solution}
    \[\]
    \vspace*{-4em}
    \begin{enumerate}[label = (\alph*)]
        \item \begin{align*}
                  v_t(x, t) & = \frac{\partial}{\partial t}u(y - ct, t)e^{at}                                                                         \\
                            & = u_t(y - ct, t)e^{at} - cu_x(y - ct, t)e^{at} + au(y - ct, t)e^{at}                                                    \\
                            & = \left(Du_{xx}(y - ct, t) + cu_x(y - ct, t) - au(y - ct, t)\right)e^{at} - cu_x(y - ct, t)e^{at} + au(y - ct, t)e^{at} \\
                            & = Du_{xx}(y - ct, t)e^{at}                                                                                              \\
                            & = Dv_{yy}(x, t)
              \end{align*}
        \item We have that \(D = 1\), \(a = 2\), and \(c = 0\). Let \(v(x, t) = u(y - ct, t)e^{at}\). Then
              \[u_t = Du_{xx} + cu_x - au \implies v_t = Dv_{yy}.\]
              Let \(y = x\), \(c = 0\), and \(a = 2\). Then
              \[v(x, t) = u(x, t)e^{2t}.\]
              \[u(x, t) = v(x, t)e^{-2t} = \frac{1}{\sqrt{4\pi t}}e^{-\frac{x^2}{4t}}e^{-2t} = \frac{1}{\sqrt{4\pi t}}e^{-\frac{x^2}{4t} - 2t}\]
    \end{enumerate}
\end{solution}


\end{document}
