\documentclass[plain]{pset}
\usepackage{dylan}

\title{Homework 3}
\author{Dylan Hu}
\prof{Professor Zhuolun Yang}
\course{APMA 0360 --- Partial Differential Equations}
\date{February 25, 2024}

\begin{document}

\begin{multicols}{2}
    \raggedcolumns{}
    \maketitle
    \columnbreak{}
    \tableofcontents
\end{multicols}

\setlength{\parskip}{1em}

\pagebreak

\begin{problem}
Solve
\[\begin{cases}\begin{aligned}
            u_t - Du_{xx} & = 0   \\
            u(x, 0)       & = e^x
        \end{aligned}\end{cases}\]
explicitly.
\begin{remark*}
    You are allowed to use the solution formula even though \(u(x, 0)\) is not in Schwartz class.
\end{remark*}
\end{problem}
\begin{solution}
    Recall that the fundamental solution to the heat equation is
    \[G(x, t) = \frac{1}{\sqrt{4\pi Dt}}e^{-\frac{x^2}{4Dt}}\]
    and the solution to the heat equation is
    \[u(x, t) = \int_{-\infty}^{\infty} G(x - y, t)u(y, 0)\,dy\]
    so
    \[u(x, t) = \frac{1}{\sqrt{4\pi Dt}} \int_{-\infty}^{\infty} e^{-\frac{{(x - y)}^2}{4Dt}}e^y\,dy.\]
    Focusing on the exponent, we have
    \[-\frac{{(x - y)}^2}{4Dt} + y = \frac{4Dty - {(x - y)}^2}{4Dt}\]
    Focusing on the numerator, we complete the square with respect to \(y\):
    \begin{align*}
        4Dty - {(x - y)}^2 & = 4Dty - x^2 + 2xy - y^2                  \\
                           & = -y^2 + 2xy + 4Dty - x^2                 \\
                           & = -y^2 + (2x + 4Dt)y - x^2                \\
                           & = -\left(y^2 - (2x + 4Dt)y\right) - x^2   \\
                           & = -{(y - x -2Dt)}^2 - x^2 + {(x + 2Dt)}^2 \\
                           & = -{(y - x - 2Dt)}^2 + 4Dtx + 4D^2t^2     \\
                           & = -{(y - x - 2Dt)}^2 + 4Dt(x + Dt)
    \end{align*}
    So we have
    \begin{align*}
        u(x, t) & = \frac{1}{\sqrt{4\pi Dt}} \int_{-\infty}^{\infty} e^{-\frac{{(y - x - 2Dt)}^2}{4Dt}}e^{x + Dt}\,dy                  \\
                & = \frac{e^{x + Dt}}{\sqrt{4\pi Dt}} \int_{-\infty}^{\infty} e^{-\frac{{(y - x - 2Dt)}^2}{4Dt}}\,dy                   \\
                & = \frac{e^{x + Dt}}{\sqrt{4\pi Dt}} \int_{-\infty}^{\infty} e^{-{\left(\frac{y - x - 2Dt}{\sqrt{4Dt}}\right)}^2}\,dy
    \end{align*}
    Let \(u = \frac{y - x - 2Dt}{\sqrt{4Dt}}\), so \(du = \frac{1}{\sqrt{4Dt}}\,dy\), and
    \[u(x, t) = \frac{e^{x + Dt}}{\sqrt{\pi}} \int_{-\infty}^{\infty} e^{-u^2}\,du\]
    which is the Gaussian integral, so
    \[u(x, t) = \frac{e^{x + Dt}}{\sqrt{\pi}} \sqrt{\pi} = e^{x + Dt}\]

\end{solution}

\pagebreak

\begin{problem}
Use the Fourier transform to find the general solution of the wave equation
\[u_{tt} = c^2u_{xx}\]
\begin{hint*}
    You may use the fact from ODE that:
    \[y'' + a^2y = 0 \implies y(t) = Ae^{iat} + Be^{-iat}\]
    and Question 1 from HW2.
\end{hint*}
\end{problem}
\begin{solution}
    We may first take the Fourier transform of both sides:
    \[\mathcal{F}\{u_{tt}\} = \mathcal{F}\{c^2u_{xx}\}\]
    \[\hat{u}_{tt} = c^2(ik)^2\hat{u}\]
    \[\hat{u}_{tt} = -c^2k^2\hat{u}\]
    This is a second order ODE in \(\hat{u}\), and we can use the provided fact to obtain
    \[\hat{u}'' + c^2k^2\hat{u} = 0 \implies \hat{u}(t) = A(k)e^{ickt} + B(k)e^{-ickt}\]
    Now we take the inverse Fourier transform of \(\hat{u}\):
    \[u(x, t) = \mathcal{F}^{-1}\{\hat{u}(t)\} = \mathcal{F}^{-1}\{Ae^{ickt} + Be^{-ickt}\}\]
    Recall from Question 1 of HW2 (using \(v\) to distinguish from \(u\)) that
    \[\hat{v}_1(k, t) = \hat{v}_1(k, 0)e^{ickt} = \hat{f_1}(k)e^{ickt} \implies v_1(x, t) = f_1(x - ct)\]
    And similarly we have
    \[\hat{v}_2(k, t) = \hat{v}_2(k, 0)e^{-ickt} = \hat{f_2}(k)e^{-ickt} \implies v_2(x, t) = f_2(x + ct)\]
    So, we may write
    \[u(x, t) = \mathcal{F}^{-1}\{A(k)e^{ickt} + B(k)e^{-ickt}\} = \mathcal{F}^{-1}\{\hat{u}(t)\} = \mathcal{F}^{-1}\{A(k)\hat{u}(k, 0)e^{ickt} + B(k)\hat{u}(k, 0)e^{-ickt}\}\]
    Letting \(f(k) \coloneqq A(k)\hat{u}(k, 0)\) and \(g(k) \coloneqq B(k)\hat{u}(k, 0)\), we have
    \[u(x, t) = \mathcal{F}^{-1}\{f(k)e^{ickt} + g(k)e^{-ickt}\} = f(x - ct) + g(x + ct)\]
\end{solution}

\pagebreak

\begin{problem}
Solve
\[\begin{cases}\begin{aligned}
            u_{tt} - 3u_{xt} - 4u_{xx} & = 0      \\
            u(x, 0)                    & = 2x^2   \\
            u_t(x, 0)                  & = e^{4x}
        \end{aligned}\end{cases}\]
\end{problem}
\begin{solution}
    % forget this, will use different method
    % We may first take the Fourier transform of both sides:
    % \[\mathcal{F}\{u_{tt}\} - 3\mathcal{F}\{u_{xt}\} - 4\mathcal{F}\{u_{xx}\} = 0\]
    % \[\hat{u}_{tt} - 3ik\hat{u}_t + 4k^2\hat{u} = 0\]
    % This is a second order ODE in \(\hat{u}\) with respect to \(t\), and we can write the auxiliary equation
    % \[r^2 - 3ikr + 4k^2 = 0\]
    % which has solutions
    % \[r = \frac{3ik \pm \sqrt{{(3ik)}^2 - 4(4k^2)}}{2} = \frac{3ik \pm \sqrt{-9k^2 - 16k^2}}{2} = \frac{3ik \pm \sqrt{-25k^2}}{2} = \frac{3ik \pm 5ik}{2} = 8ik, -ik\]
    % So we have

    \[u_{tt} - 3u_{xt} - 4u_{xx} \Longleftrightarrow \left(\frac{\partial}{\partial t} - 4\frac{\partial }{\partial x}\right)\left(\frac{\partial }{\partial t} + \frac{\partial }{\partial x}\right)u = 0\]
    So we have
    \[\begin{cases}\begin{aligned}
                \xi  & = x - t  \\
                \eta & = x + 4t
            \end{aligned}\end{cases}\]
    and \[\begin{cases}\begin{aligned}
                x & = \frac{4\xi + \eta}{5} \\
                t & = \frac{\eta - \xi}{5}
            \end{aligned}\end{cases}\]
    Then
    \[\frac{\partial }{\partial \xi} = \frac{4}{5}\frac{\partial }{\partial x} - \frac{1}{5}\frac{\partial }{\partial t} = -\frac{1}{5}\left(\frac{\partial }{\partial t} - 4\frac{\partial }{\partial x}\right)\]
    and
    \[\frac{\partial }{\partial \eta} = \frac{1}{5}\frac{\partial }{\partial x} + \frac{1}{5}\frac{\partial }{\partial t} = \frac{1}{5}\left(\frac{\partial }{\partial t} + \frac{\partial }{\partial x}\right)\]
    Let us define
    \[V(\xi, \eta) = u\left(\frac{4\xi + \eta}{5}, \frac{\eta - \xi}{5}\right)\]
    As in lecture, we can compute to find
    \[V_{\xi\eta} = 0 \implies V(\xi, \eta) = F(\xi) + G(\eta) = F(x - t) + G(x + 4t)\]
    so
    \[u(x, t) = F(x - t) + G(x + 4t)\]
    Now we need to find \(F\) and \(G\) using the initial conditions.



\end{solution}

\pagebreak

\begin{problem}
Choose \(\alpha > 0\). Let \(u(x, t)\) be a solution of Schwartz to the damped wave equation \(u_{tt} + \alpha u_t = u_{xx}\). Show that the energy
\[E(t) = \frac{1}{2}\int_{-\infty}^{\infty} \left[{\left(u_t(x, t)\right)}^2 + {\left(u_x(x, t)\right)}^2\right]dx\]
is non-increasing (\(\frac{d}{dt}E(t) \leq 0\)).
\end{problem}
\begin{solution}
    \begin{align*}
        \frac{d}{dt}E(t) & = \frac{1}{2}\int_{-\infty}^{\infty} \frac{\partial }{\partial t}\left[{\left(u_t(x, t)\right)}^2 + {\left(u_x(x, t)\right)}^2\right]dx                            \\
                         & = \frac{1}{2}\int_{-\infty}^{\infty} 2u_t(x, t)u_{tt}(x, t) + 2u_x(x, t)u_{xt}(x, t)dx                                                                             \\
                         & = \int_{-\infty}^{\infty} u_t(x, t)(u_{xx}(x, t) - \alpha u_t(x, t)) + u_x(x, t)u_{xt}(x, t)dx                                                                     \\
                         & = \int_{-\infty}^{\infty} u_t(x, t)u_{xx}(x, t) dx - \alpha \int_{-\infty}^{\infty} {\left(u_t(x, t)\right)}^2dx + \int_{-\infty}^{\infty} u_x(x, t)u_{xt}(x, t)dx \\
                         & = -\int_{-\infty}^{\infty} u_x(x, t)u_t(x, t)dx - \alpha \int_{-\infty}^{\infty} {\left(u_t(x, t)\right)}^2dx + \int_{-\infty}^{\infty} u_x(x, t)u_{xt}(x, t)dx    \\
                         & = -\int_{-\infty}^{\infty} u_x(x, t)u_{xt}(x, t)dx - \alpha \int_{-\infty}^{\infty} {\left(u_t(x, t)\right)}^2dx + \int_{-\infty}^{\infty} u_x(x, t)u_{xt}(x, t)dx \\
                         & = -\alpha \int_{-\infty}^{\infty} {\left(u_t(x, t)\right)}^2dx \leq 0
    \end{align*}
    where the last inequality follows from the fact that \(\alpha > 0\) and the integrand is non-negative.
\end{solution}


\end{document}
